hol/p4_from_json/concurrency_tests/concur1_interferenceScript.sml
@@ -1,22 +1,11 @@
 open HolKernel Parse bossLib boolSyntax;
 open p4_testLib p4_arch_auxTheory;
-open p4_concurrentTheory;
+open p4_concurrentTheory p4_v1modelTheory;
+open bitstringTheory;
 
-val _ = new_theory "concur1_interleaving";
+open pairSyntax p4Syntax p4_concurrentSyntax p4_v1modelLib;
 
-(*
-(stmt_ass lval_null
-            (e_call (funn_inst "register")
-               [e_var (varn_name "r");
-                e_v
-                  (v_bit
-                     ([F; F; F; F; F; F; F; F; F; F; F; F; F; F; F; F; F; F;
-                       F; F; F; F; F; F; F; F; F; F; F; F; F; T],32));
-                e_v
-                  (v_bit
-                     ([ARB; ARB; ARB; ARB; ARB; ARB; ARB; ARB; ARB; ARB; ARB;
-                       ARB; ARB; ARB; ARB; ARB],16))]))
-*)
+val _ = new_theory "concur1_interference";
 
 val concur1_actx = ``([arch_block_inp;
   arch_block_pbl "MyParser"
@@ -121,12 +110,12 @@ val concur1_actx = ``([arch_block_inp;
 
 val concur1_astate =
  ``((0, (* Block index *)
-     [([T], 1)], (* Input list *)
+     [([T], 1:num); ([F], 2)], (* Input list *)
      [], (* Output list *)
      (* 'a: *)
      1, (* Number of extern objects *)
      [(0, INR (v1model_v_ext_register [(fixwidth 16 [], 16)]))],
-     ["r", v_ext_ref 0],
+     (^v1model_init_v_map++["r", v_ext_ref 0]),
      [("flowlet",[]); ("new_flowlet",[])]), (* End of 'a env *)
     [[(varn_name "r", (v_ext_ref 0, NONE))]], (* g_scope_list *)
     arch_frame_list_empty, (* frame_list *)
@@ -134,12 +123,12 @@ val concur1_astate =
    ):v1model_ascope astate``;
 
 val concur1_shared_s =
- ``([([T], 1:num)], (* Input list *)
+ ``([([T], 1:num); ([F], 2)], (* Input list *)
     []: (bool list # num) list, (* Output list *)
     (* 'a: *)
     (1:num, (* Number of extern objects *)
      [(0:num, INR (v1model_v_ext_register [(fixwidth 16 [], 16)]))]:(num # (core_v_ext + v1model_v_ext)) list,
-     ["r", v_ext_ref 0],
+     (^v1model_init_v_map++["r", v_ext_ref 0]),
      [("flowlet",[]:(e list # string # e list) list); ("new_flowlet",[])])
    )``;
 
@@ -156,24 +145,6 @@ val concur1_t2_s =
     arch_frame_list_empty,
     status_running
    )``;
-
-Definition v1model_ascope_read_ext_obj_def:
- v1model_ascope_read_ext_obj ((counter, ext_obj_map, v_map, ctrl):v1model_ascope) vname =
-  case ALOOKUP v_map vname of
-  | SOME (v_ext_ref n) =>
-   ALOOKUP ext_obj_map n
-  | _ => NONE
-End
-
-Definition v1model_ascope_of_conc_state_def:
- v1model_ascope_of_conc_state (io1,io2,(ascope:v1model_ascope)) =
-  ascope
-End
-
-Definition p4_finished_def:
- p4_finished ((io1 ,io2 , a), ((i1, gsl1, framel1, status1), (i2, gsl2, framel2, status2))) =
-  (io1 = [] /\ status1 = status_running /\ status2 = status_running)
-End
 
 (*
 (* 28 steps to finishing first function *)
@@ -194,66 +165,125 @@ Second witness from
 
  val (_, ((i, _, in_out_list', _), g_scope_list, arch_frame_list, status)) = debug_arch_from_step "v1model" concur1_actx concur1_astate 55
 *)
- val (_, ((i1', _, _, _), g_scope_list1', arch_frame_list1', status1')) = debug_arch_from_step "v1model" concur1_actx concur1_astate 55
+
+val (_, ((i1', _, _, _), g_scope_list1', arch_frame_list1', status1')) = debug_arch_from_step "v1model" concur1_actx concur1_astate 55
 
 val t1_s' = “(0:num, ^g_scope_list1', arch_frame_list_empty, status_running)”;
 val t2_s' = “(0:num, ^g_scope_list1', arch_frame_list_empty, status_running)”;
 
- val (_, ((_, io_list, io_list', ascope'), _, _, _)) = debug_arch_from_step "v1model" concur1_actx concur1_astate 55
+(*
+val (_, ((_, io_list, io_list', ascope'), _, _, _)) = debug_arch_from_step "v1model" concur1_actx concur1_astate 55
+*)
 
-val shared_s' = “(^io_list, ^io_list', ^ascope')”;
+val shared_s'_standard_metadata =
+ listSyntax.mk_list
+  (map pairSyntax.mk_pair
+   [(``"ingress_port"``, mk_v_bitii (2, 9)),
+    (``"egress_spec"``, mk_v_bitii (0, 9)),
+    (``"egress_port"``, mk_v_bitii (0, 9)),
+    (``"instance_type"``, mk_v_bitii (0, 32)),
+    (``"packet_length"``, mk_v_bitii (0, 32)),
+    (``"enq_timestamp"``, mk_v_bitii (0, 32)),
+    (``"enq_qdepth"``, mk_v_bitii (0, 19)),
+    (``"deq_timedelta"``, mk_v_bitii (0, 32)),
+    (``"deq_qdepth"``, mk_v_bitii (0, 19)),
+    (``"ingress_global_timestamp"``, mk_v_bitii (0, 48)),
+    (``"egress_global_timestamp"``, mk_v_bitii (0, 48)),
+    (``"mcast_grp"``, mk_v_bitii (0, 16)),
+    (``"egress_rid"``, mk_v_bitii (0, 16)),
+    (``"checksum_error"``, mk_v_bitii (0, 1)),
+    (``"parser_error"``, mk_v_bitii (0, 32)),
+    (``"priority"``, mk_v_bitii (0, 3))],
+   “:(string # v)”);
+val shared_s' =
+“([]:(bool list # num) list,[([F], 0:num); ([F], 0)],5:num,
+  [(0:num,INR (v1model_v_ext_register [(w2v (1w:word16),16)]));
+   (1,INL (core_v_ext_packet [])); (2,INL (core_v_ext_packet [T]));
+   (3,INL (core_v_ext_packet [])); (4,INL (core_v_ext_packet [F]))],
+  [("parseError",v_bit (w2v (0w:word32),32)); ("r",v_ext_ref 0); ("b",v_ext_ref 3);
+   ("b_temp",v_ext_ref 4);
+   ("standard_metadata",
+    v_struct ^shared_s'_standard_metadata);
+   ("parsedHdr",v_struct []); ("hdr",v_struct []); ("meta",v_struct [])],
+  [("flowlet",[]:(e list # string # e list) list); ("new_flowlet",[])])”;
+
 val shared_s'' =
-   “([]:(bool list # num) list,[([T],0:num)],3:num,
-     [(0:num,INR (v1model_v_ext_register [(w2v 2w,16)]));
-      (1,INL (core_v_ext_packet [])); (2,INL (core_v_ext_packet [T]))],
-     [("parseError",v_bit (w2v 0w,32)); ("b",v_ext_ref 1);
-      ("b_temp",v_ext_ref 2);
-      ("standard_metadata",
-       v_struct
-         [("ingress_port",v_bit (w2v 1w,9));
-          ("egress_spec",v_bit (w2v 0w,9)); ("egress_port",v_bit (w2v 0w,9));
-          ("instance_type",v_bit (w2v 0w,32));
-          ("packet_length",v_bit (w2v 0w,32));
-          ("enq_timestamp",v_bit (w2v 0w,32));
-          ("enq_qdepth",v_bit (w2v 0w,19));
-          ("deq_timedelta",v_bit (w2v 0w,32));
-          ("deq_qdepth",v_bit (w2v 0w,19));
-          ("ingress_global_timestamp",v_bit (w2v 0w,48));
-          ("egress_global_timestamp",v_bit (w2v 0w,48));
-          ("mcast_grp",v_bit (w2v 0w,16)); ("egress_rid",v_bit (w2v 0w,16));
-          ("checksum_error",v_bit (w2v 0w,1));
-          ("parser_error",v_bit (w2v 0w,32)); ("priority",v_bit (w2v 0w,3))]);
-      ("parsedHdr",v_struct []); ("hdr",v_struct []); ("meta",v_struct [])],
-     [("flowlet",[]:(e list # string # e list) list); ("new_flowlet",[])])”;
+“([]:(bool list # num) list,[([T], 0:num); ([F], 0)],5:num,
+  [(0:num,INR (v1model_v_ext_register [(w2v (2w:word16),16)]));
+   (1,INL (core_v_ext_packet [])); (2,INL (core_v_ext_packet [T]));
+   (3,INL (core_v_ext_packet [])); (4,INL (core_v_ext_packet [F]))],
+  [("parseError",v_bit (w2v (0w:word32),32)); ("r",v_ext_ref 0); ("b",v_ext_ref 3);
+   ("b_temp",v_ext_ref 4);
+   ("standard_metadata",
+    v_struct ^shared_s'_standard_metadata);
+   ("parsedHdr",v_struct []); ("hdr",v_struct []); ("meta",v_struct [])],
+  [("flowlet",[]:(e list # string # e list) list); ("new_flowlet",[])])”;
 
-(* TODO: You can be more specific about what differs in the two traces *)
-(* TODO: Fix t1_s, t2_s and shared_s to align with the concur1 example *)
+val init_conc_state = list_mk_pair[concur1_shared_s, concur1_t1_s, concur1_t2_s];
+
+val trace1_thm =
+ let
+  val thm1 = get_trace_thread_n "v1model" concur1_actx init_conc_state 28 1
+  val thm2 = get_trace_thread_next_n "v1model" concur1_actx thm1 28 2
+  val thm3 = get_trace_thread_next_n "v1model" concur1_actx thm2 27 1
+  val thm4 = get_trace_thread_next_n "v1model" concur1_actx thm3 27 2
+ in
+  thm4
+ end;
+
+val trace2_thm =
+ let
+  (* Call 1: to get_trace_thread_n *)
+  val thm1 = get_trace_thread_n "v1model" concur1_actx init_conc_state 55 1
+
+  (* Call 2: Should be to a new to get_trace_thread_next_n that continues from a theorem *)
+  val thm2 = get_trace_thread_next_n "v1model" concur1_actx thm1 55 2
+ in
+  thm2
+ end;
+
 Theorem concur1_trace_path_interference:
  ?n t1_s' t2_s' shared_s' shared_s''.
   (trace_path ( \s s'. conc_red ^concur1_actx s s') n (^concur1_shared_s, (^concur1_t1_s, ^concur1_t2_s))
                                             (shared_s', (t1_s', t2_s')) /\
-   p4_finished (shared_s', (t1_s', t2_s')) /\
+   p4_conc_finished (shared_s', (t1_s', t2_s')) /\
    v1model_ascope_read_ext_obj (v1model_ascope_of_conc_state shared_s') "r" =
     SOME (INR (v1model_v_ext_register [(fixwidth 16 (n2v 1), 16)]))) /\
   (trace_path ( \s s'. conc_red ^concur1_actx s s') n (^concur1_shared_s, (^concur1_t1_s, ^concur1_t2_s))
                                             (shared_s'', (t1_s', t2_s')) /\
-   p4_finished (shared_s'', (t1_s', t2_s')) /\
-   v1model_ascope_read_ext_obj (v1model_ascope_of_conc_state shared_s') "r" =
+   p4_conc_finished (shared_s'', (t1_s', t2_s')) /\
+   v1model_ascope_read_ext_obj (v1model_ascope_of_conc_state shared_s'') "r" =
     SOME (INR (v1model_v_ext_register [(fixwidth 16 (n2v 2), 16)])))
 Proof
-EXISTS_TAC “55:num” >>
+EXISTS_TAC “110:num” >>
 EXISTS_TAC t1_s' >>
 EXISTS_TAC t2_s' >>
 EXISTS_TAC shared_s' >>
 EXISTS_TAC shared_s'' >>
 CONJ_TAC >| [
- (* 1. For witness of r=1, t1 executes the first function, then t2 executes the first function, then t1 the rest, then t2 the rest. *)
- cheat,
+ rpt strip_tac >| [
+  (* 1. For witness of r=1, t1 executes the first function, then t2 executes the first function, then t1 the rest, then t2 the rest. *)
+  ASSUME_TAC trace1_thm >>
+  gvs [w2v_def],
 
- (* 2. For witness of r=2, use executable semantics, then arch_exec_trace_n,
-  * then arch_path_implies_conc_thread1, then executable semantics for thread 2, then
-  * arch_exec_trace_n, then arch_path_implies_conc_thread2, then conc_paths_compose. *)
- cheat
+  fs[p4_conc_finished_def],
+
+  fs[v1model_ascope_of_conc_state_def, v1model_ascope_read_ext_obj_def] >>
+  EVAL_TAC
+ ],
+
+ rpt strip_tac >| [
+  (* 2. For witness of r=2, use executable semantics, then arch_exec_trace_n,
+   * then arch_path_implies_conc_thread1, then executable semantics for thread 2, then
+   * arch_exec_trace_n, then arch_path_implies_conc_thread2, then conc_paths_compose. *)
+  ASSUME_TAC trace2_thm >>
+  gvs [w2v_def],
+
+  fs[p4_conc_finished_def],
+
+  fs[v1model_ascope_of_conc_state_def, v1model_ascope_read_ext_obj_def] >>
+  EVAL_TAC
+ ]
 ]
 QED
 
