hol/p4_exec_semScript.sml
@@ -2439,7 +2439,14 @@ Theorem arch_multi_exec_1:
 !actx s s'.
  arch_multi_exec actx s 1 = SOME s' <=> arch_exec actx s = SOME s'
 Proof
-cheat
+rpt strip_tac >>
+PairCases_on ‘s’ >>
+REWRITE_TAC [arithmeticTheory.ONE, arch_multi_exec] >>
+Cases_on ‘arch_exec actx ((s0,s1,s2,s3),s4,s5,s6)’ >> (
+ fs[]
+) >>
+PairCases_on ‘x’ >>
+fs[]
 QED
 
 Theorem arch_multi_exec_add:
